migrating to trimmed down MR interface

src/tls/StreamAE.fst
@@ -105,10 +105,10 @@ let genPost (#i:id) parent h0 (w:writer i) h1 =
   fresh_region (AEAD.region w.aead) h0 h1 /\
   color (AEAD.region w.aead) = color parent /\
   (authId i ==>
-      (m_contains (ilog w.log) h1 /\
-       m_sel h1 (ilog w.log) == createEmpty)) /\
-  m_contains (ctr w.counter) h1 /\
-  m_sel h1 (ctr w.counter) === 0
+      (HS.contains h1 (ilog w.log) /\
+       HS.sel h1 (ilog w.log) == createEmpty)) /\
+  HS.contains h1 (ctr w.counter) /\
+  HS.sel h1 (ctr w.counter) === 0
 //16-04-30 how to share the whole ST ... instead of genPost?
 
 // Generate a fresh instance with index i in a fresh sub-region of r0
@@ -129,7 +129,7 @@ let gen parent i =
     let ectr: ideal_ctr #writer_r writer_r i log = new_seqn #writer_r #(entry i) #max_ctr writer_r 0 log in
     State #i #Writer #writer_r #writer_r aead log ectr
   else
-    let ectr: concrete_ctr writer_r i = m_alloc writer_r 0 in
+    let ectr: concrete_ctr writer_r i = ralloc writer_r 0 in
     State #i #Writer #writer_r #writer_r aead () ectr
 
 #reset-options
@@ -143,8 +143,8 @@ val genReader: parent:rgn -> #i:id -> w:writer i -> ST (reader i)
 	       color r.region = color parent /\
          fresh_region r.region h0 h1 /\
          w.log == r.log /\
-	 m_contains (ctr r.counter) h1 /\
-	 m_sel h1 (ctr r.counter) === 0))
+	 HS.contains h1 (ctr r.counter) /\
+	 HS.sel h1 (ctr r.counter) === 0))
 // encryption (on concrete bytes), returns (cipher @| tag)
 // Keeps seqn and nonce implicit; requires the counter not to overflow
 // encryption of plaintexts; safe instances are idealized
@@ -160,7 +160,7 @@ let genReader parent #i w =
     let log : ideal_log w.region i = w.log in
     let dctr: ideal_ctr reader_r i log = new_seqn reader_r 0 log in
     State #i #Reader #reader_r #writer_r raead w.log dctr
-  else let dctr : concrete_ctr reader_r i = m_alloc reader_r 0 in
+  else let dctr : concrete_ctr reader_r i = ralloc reader_r 0 in
     State #i #Reader #reader_r #writer_r raead () dctr
 
 // Coerce a writer with index i in a fresh subregion of parent
@@ -172,7 +172,7 @@ val coerce: parent:rgn -> i:id{~(authId i)} -> kv:key i -> iv:iv i -> ST (writer
 let coerce parent i kv iv =
   assume false; // coerce missing post-condition
   let writer_r = new_region parent in
-  let ectr: concrete_ctr writer_r i = m_alloc writer_r 0 in
+  let ectr: concrete_ctr writer_r i = ralloc writer_r 0 in
   let aead = AEAD.coerce i parent kv iv in
   State #i #Writer #writer_r #writer_r aead () ectr
 
@@ -196,19 +196,19 @@ val encrypt: #i:id -> e:writer i -> l:plainLen -> p:plain i l -> ST (cipher i l)
       lemma_ID13 i;
       HS.disjoint e.region (AEAD.log_region #i e.aead) /\
       l <= max_TLSPlaintext_fragment_length /\ // FIXME ADL: why is plainLen <= max_TLSCiphertext_fragment_length_13 ?? Fix StreamPlain!
-      m_sel h0 (ctr e.counter) < max_ctr))
+      HS.sel h0 (ctr e.counter) < max_ctr))
     (ensures  (fun h0 c h1 ->
       lemma_ID13 i;
       modifies (Set.as_set [e.log_region; AEAD.log_region #i e.aead]) h0 h1 /\
-      m_contains (ctr e.counter) h1 /\
-      m_sel h1 (ctr e.counter) === m_sel h0 (ctr e.counter) + 1 /\
+      HS.contains h1 (ctr e.counter) /\
+      HS.sel h1 (ctr e.counter) === HS.sel h0 (ctr e.counter) + 1 /\
 	    (authId i ==>
 		    (let log = ilog e.log in
 		    let ent = Entry l c p in
-		    let n = Seq.length (m_sel h0 log) in
-		    m_contains log h1 /\
-		    Monotonic.RRef.witnessed (at_least n ent log) /\
-		    m_sel h1 log == snoc (m_sel h0 log) ent))))
+		    let n = Seq.length (HS.sel h0 log) in
+		    HS.contains h1 log /\
+		    witnessed (at_least n ent log) /\
+		    HS.sel h1 log == snoc (HS.sel h0 log) ent))))
 
 (* we primarily model the ideal functionality, the concrete code that actually
    runs on the network is what remains after dead code elimination when
@@ -218,9 +218,9 @@ val encrypt: #i:id -> e:writer i -> l:plainLen -> p:plain i l -> ST (cipher i l)
 let encrypt #i e l p =
   let h0 = get() in
   let ctr = ctr e.counter in
-  m_recall ctr;
+  recall ctr;
   let text = if safeId i then createBytes l 0z else repr i l p in
-  let n = m_read ctr in
+  let n = !ctr in
   lemma_repr_bytes_values n;
   let nb = bytes_of_int (AEAD.noncelen i) n in
   let iv = AEAD.create_nonce e.aead nb in
@@ -231,16 +231,16 @@ let encrypt #i e l p =
   if authId i then
     begin
     let ilog = ilog e.log in
-    m_recall ilog;
+    recall ilog;
     let ictr: ideal_ctr e.region i ilog = e.counter in
     testify_seqn ictr;
     write_at_end ilog (Entry l c p); //need to extend the log first, before incrementing the counter for monotonicity; do this only if ideal
-    m_recall ictr;
+    recall ictr;
     increment_seqn ictr;
-    m_recall ictr
+    recall ictr
     end
   else
-    m_write ctr (n + 1);
+    ctr := (n + 1);
   c
 
 (* val matches: #i:id -> l:plainLen -> cipher i l -> entry i -> Tot bool *)
@@ -253,20 +253,20 @@ val decrypt: #i:id -> d:reader i -> l:plainLen -> c:cipher i l
   -> ST (option (plain i (min l (max_TLSPlaintext_fragment_length + 1))))
   (requires (fun h0 ->
      l <= max_TLSPlaintext_fragment_length /\ // FIXME ADL: why is plainLen <= max_TLSCiphertext_fragment_length_13 ?? Fix StreamPlain!
-     m_sel h0 (ctr d.counter) < max_ctr))
+     HS.sel h0 (ctr d.counter) < max_ctr))
   (ensures  (fun h0 res h1 ->
-      let j : nat = m_sel h0 (ctr d.counter) in
+      let j : nat = HS.sel h0 (ctr d.counter) in
       (authId i ==>
-    	(let log = m_sel h0 (ilog d.log) in
+    	(let log = HS.sel h0 (ilog d.log) in
     	 if j < Seq.length log && matches l c (Seq.index log j)
     	 then res = Some (Entry?.p (Seq.index log j))
     	 else res = None)) /\
       (match res with
        | None -> HS.modifies_transitively Set.empty h0 h1
-       | _ -> let ctr_counter_as_hsref = as_hsref (ctr d.counter) in
+       | _ -> let ctr_counter_as_hsref = ctr d.counter in
              HS.modifies_one d.region h0 h1 /\
              modifies_ref d.region (Set.singleton (Heap.addr_of (as_ref ctr_counter_as_hsref))) h0 h1 /\
-             m_sel h1 (ctr d.counter) === j + 1)))
+             HS.sel h1 (ctr d.counter) === j + 1)))
 
 val strip_refinement: #a:Type -> #p:(a -> Type0) -> o:option (x:a{p x}) -> option a
 let strip_refinement #a #p = function
@@ -277,18 +277,18 @@ let strip_refinement #a #p = function
 // decryption, idealized as a lookup of (c,ad) in the log for safe instances
 let decrypt #i d l c =
   let ctr = ctr d.counter in
-  m_recall ctr;
-  let j = m_read ctr in
+  recall ctr;
+  let j = !ctr in
   if authId i
   then
     let ilog = ilog d.log in
-    let log  = m_read ilog in
+    let log  = !ilog in
     let ictr: ideal_ctr d.region i ilog = d.counter in
     let _ = testify_seqn ictr in //now we know that j <= Seq.length log
     if j < Seq.length log && matches l c (Seq.index log j) then
       begin
       increment_seqn ictr;
-      m_recall ctr;
+      recall ctr;
       Some (Entry?.p (Seq.index log j))
       end
     else None
@@ -305,7 +305,7 @@ let decrypt #i d l c =
      begin
        assert (Platform.Bytes.length pr == l);
        let p = strip_refinement (mk_plain i l pr) in
-       if Some? p then m_write ctr (j + 1);
+       if Some? p then ctr := (j + 1);
        p
      end
    end
