src/tls/PSK.fst
@@ -64,10 +64,10 @@ private let app_psk_table : MM.t psk_region psk_identifier app_psk_entry psk_tab
   MM.alloc #psk_region #psk_identifier #app_psk_entry #psk_table_invariant
 
 abstract type registered_psk (i:psk_identifier) =
-  MR.witnessed (MM.defined app_psk_table i)
+  witnessed (MM.defined app_psk_table i)
 
 let valid_app_psk (ctx:pskInfo) (i:psk_identifier) (h:mem) =
-  match MM.sel (MR.m_sel h app_psk_table) i with
+  match MM.sel (sel h app_psk_table) i with
   | Some (_, c, _) -> b2t (c = ctx)
   | _ -> False
 
@@ -77,7 +77,7 @@ let psk_value (i:pskid) : ST (app_psk i)
   (requires (fun h0 -> True))
   (ensures (fun h0 _ h1 -> modifies_none h0 h1))
   =
-  MR.m_recall app_psk_table;
+  recall app_psk_table;
   MR.testify (MM.defined app_psk_table i);
   match MM.lookup app_psk_table i with
   | Some (psk, _, _) -> psk
@@ -86,7 +86,7 @@ let psk_info (i:pskid) : ST (pskInfo)
   (requires (fun h0 -> True))
   (ensures (fun h0 _ h1 -> modifies_none h0 h1))
   =
-  MR.m_recall app_psk_table;
+  recall app_psk_table;
   MR.testify (MM.defined app_psk_table i);
   match MM.lookup app_psk_table i with
   | Some (_, ctx, _) -> ctx
@@ -97,7 +97,7 @@ let psk_lookup (i:psk_identifier) : ST (option pskInfo)
     modifies_none h0 h1
     /\ (Some? r ==> registered_psk i)))
   =
-  MR.m_recall app_psk_table;
+  recall app_psk_table;
   match MM.lookup app_psk_table i with
   | Some (_, ctx, _) ->
     assume(MR.stable_on_t app_psk_table (MM.defined app_psk_table i));
@@ -109,7 +109,7 @@ type honest_st (i:pskid) (h:mem) =
   (MM.defined app_psk_table i h /\
   (let (_,_,b) = MM.value app_psk_table i h in b = true))
 
-type honest_psk (i:pskid) = MR.witnessed (honest_st i)
+type honest_psk (i:pskid) = witnessed (honest_st i)
 
 // Generates a fresh PSK identity
 val fresh_psk_id: unit -> ST psk_identifier
@@ -133,14 +133,14 @@ let gen_psk (i:psk_identifier) (ctx:pskInfo)
     registered_psk i /\
     honest_psk i))
   =
-  MR.m_recall app_psk_table;
+  recall app_psk_table;
   let psk = (abyte 1z) @| CoreCrypto.random 32 in
   assume(index psk 0 = 1z);
   let add : app_psk_entry i = (psk, ctx, true) in
   MM.extend app_psk_table i add;
   MM.contains_stable app_psk_table i add;
   let h = get () in
-  cut(MM.sel (MR.m_sel h app_psk_table) i == Some add);
+  cut(MM.sel (sel h app_psk_table) i == Some add);
   assume(MR.stable_on_t app_psk_table (honest_st i));
   MR.witness app_psk_table (honest_st i)
 
@@ -152,12 +152,12 @@ let coerce_psk (i:psk_identifier) (ctx:pskInfo) (k:app_psk i)
     registered_psk i /\
     ~(honest_psk i)))
   =
-  MR.m_recall app_psk_table;
+  recall app_psk_table;
   let add : app_psk_entry i = (k, ctx, false) in
   MM.extend app_psk_table i add;
   MM.contains_stable app_psk_table i add;
   let h = get () in
-  cut(MM.sel (MR.m_sel h app_psk_table) i == Some add);
+  cut(MM.sel (sel h app_psk_table) i == Some add);
   admit()
 
 abstract let compatible_hash_ae_st (i:pskid) (ha:hash_alg) (ae:aeadAlg) (h:mem) =
@@ -166,21 +166,21 @@ abstract let compatible_hash_ae_st (i:pskid) (ha:hash_alg) (ae:aeadAlg) (h:mem) 
   ha = pskInfo_hash ctx /\ ae = pskInfo_ae ctx))
 
 let compatible_hash_ae (i:pskid) (h:hash_alg) (a:aeadAlg) =
-  MR.witnessed (compatible_hash_ae_st i h a)
+  witnessed (compatible_hash_ae_st i h a)
 
 abstract let compatible_info_st (i:pskid) (c:pskInfo) (h:mem) =
   (MM.defined app_psk_table i h /\
   (let (_,ctx,_) = MM.value app_psk_table i h in c = ctx))
 
 let compatible_info (i:pskid) (c:pskInfo) =
-  MR.witnessed (compatible_info_st i c)
+  witnessed (compatible_info_st i c)
 
 let verify_hash_ae (i:pskid) (ha:hash_alg) (ae:aeadAlg) : ST bool
   (requires (fun h0 -> True))
   (ensures (fun h0 b h1 ->
     b ==> compatible_hash_ae i ha ae))
   =
-  MR.m_recall app_psk_table;
+  recall app_psk_table;
   MR.testify (MM.defined app_psk_table i);
   match MM.lookup app_psk_table i with
   | Some x ->
